rewrote the soundness proof

backend/AliasMemMap.v
@@ -15,4 +15,26 @@ Module MemMap <: PTMap.
 
   Axiom add : aloc -> PTSet.t -> t -> t.
 
+  Definition ge m m' :=
+    forall key, PTSet.ge (get key m) (get key m').
+
+  Axiom ge_refl : forall m, ge m m.
+
+  Axiom ge_trans : forall a b c, ge a b -> ge b c -> ge a c.
+
+  Axiom ge_add: forall k v m, ge (add k v m) m.
+
+  Axiom get_ge: forall m m',
+    ge m m' ->
+    (forall k, PTSet.ge (get k m) (get k m')).
+
+  Axiom get_add_same: forall k v m, PTSet.ge (get k (add k v m)) v.
+
+  Axiom get_top: forall k, PTSet.ge (get k top) PTSet.top.
+
+  Axiom ge_top : forall m, ge top m.
+
+  (* specific to MemMap *)
+  Axiom get_add_lt : forall x y s m, aloc_lt x y -> PTSet.ge (get x (add y s m)) s.
+
 End MemMap.
