backend/AliasPTMap.v
@@ -2,9 +2,9 @@ Require Export AliasPTSet.
 
 Module Type PTMap.
 
-  Parameter k : Type.
+  Parameter Inline k : Type.
 
-  Parameter t : Type.
+  Parameter Inline t : Type.
 
   Parameter top : t.
 
@@ -13,5 +13,24 @@ Module Type PTMap.
   Parameter get : k -> t -> PTSet.t.
 
   Parameter add : k -> PTSet.t -> t -> t.
+
+  Definition ge m m' :=
+    forall key, PTSet.ge (get key m) (get key m').
+
+  Axiom ge_refl : forall m, ge m m.
+
+  Axiom ge_trans : forall a b c, ge a b -> ge b c -> ge a c.
+
+  Axiom ge_add : forall k v m, ge (add k v m) m.
+
+  Axiom get_ge : forall m m',
+    ge m m' ->
+    (forall k, PTSet.ge (get k m) (get k m')).
+
+  Axiom get_add_same : forall k v m, PTSet.ge (get k (add k v m)) v.
+
+  Axiom get_top : forall k, PTSet.ge (get k top) PTSet.top.
+
+  Axiom ge_top : forall m, ge top m.
 
 End PTMap.
