backend/AliasPTSet.v
@@ -2,23 +2,65 @@ Require Import AliasAbstract.
 
 Module Type PTSetT.
 
-  Parameter t : Set.
+  Definition elt := aloc.
+
+  Parameter Inline t : Set.
 
   Parameter bot : t.
 
   Parameter top : t.
 
-  Parameter add : aloc -> t -> t.
+  Parameter add : elt -> t -> t.
 
-  Parameter singleton : aloc -> t.
+  Parameter singleton : elt -> t.
 
-  Parameter fold : forall {x}, (aloc -> x -> x) -> t -> x -> x.
+  Parameter fold : forall {x}, (elt -> x -> x) -> t -> x -> x.
 
   Parameter join : t -> t -> t.
+
+  Parameter In : elt -> t -> Prop.
+
+  Axiom In_add : forall x s, In x s -> forall y, In x (add y s).
+
+  Axiom In_add_same : forall x s, In x (add x s).
+
+  Axiom In_add_lt : forall x y s, aloc_lt x y -> In x (add y s).
+
+  Axiom fold_preserves_prop:
+    forall S (P : S -> Prop) (f : _ -> S -> S) s x,
+      P x ->
+      (forall x y, P x -> P (f y x)) ->
+      P (fold f s x).
+
+  Axiom fold_adds_prop:
+    forall S (P : S -> Prop) (f : _ -> S -> S) e s x,
+      In e s ->
+      (forall x, P (f e x)) ->
+      (forall x y, P x -> P (f y x)) ->
+      P (fold f s x).
+
+  Axiom In_top : forall x, In x top.
+
+  Axiom In_singleton : forall x, In x (singleton x).
+
+  Definition ge s s' :=
+    forall elt, In elt s' -> In elt s.
+
+  Axiom ge_refl : forall s, ge s s.
+
+  Axiom ge_trans : forall a b c, ge a b -> ge b c -> ge a c.
+
+  Axiom ge_join_l : forall a b, ge (join a b) a.
+
+  Axiom ge_join_r : forall a b, ge (join a b) b.
+
+  Axiom loc_In_add_blk : forall b o s, In (Loc b o) (add (Blk b) s).
 
 End PTSetT.
 
 Module PTSet <: PTSetT.
+
+  Definition elt := aloc.
 
   Axiom t : Set.
 
@@ -33,5 +75,43 @@ Module PTSet <: PTSetT.
   Axiom fold : forall {x}, (aloc -> x -> x) -> t -> x -> x.
 
   Axiom join : t -> t -> t.
+
+  Axiom In : elt -> t -> Prop.
+
+  Axiom In_add : forall x s, In x s -> forall y, In x (add y s).
+
+  Axiom In_add_same : forall x s, In x (add x s).
+
+  Axiom In_add_lt : forall x y s, aloc_lt x y -> In x (add y s).
+
+  Axiom fold_preserves_prop:
+    forall S (P : S -> Prop) (f : _ -> S -> S) s x,
+      P x ->
+      (forall x y, P x -> P (f y x)) ->
+      P (fold f s x).
+
+  Axiom fold_adds_prop:
+    forall S (P : S -> Prop) (f : _ -> S -> S) e s x,
+      In e s ->
+      (forall x, P (f e x)) ->
+      (forall x y, P x -> P (f y x)) ->
+      P (fold f s x).
+
+  Axiom In_top : forall x, In x top.
+
+  Axiom In_singleton : forall x, In x (singleton x).
+
+  Definition ge s s' :=
+    forall elt, In elt s' -> In elt s.
+
+  Axiom ge_refl : forall s, ge s s.
+
+  Axiom ge_trans : forall a b c, ge a b -> ge b c -> ge a c.
+
+  Axiom ge_join_l : forall a b, ge (join a b) a.
+
+  Axiom ge_join_r : forall a b, ge (join a b) b.
+
+  Axiom loc_In_add_blk : forall b o s, In (Loc b o) (add (Blk b) s).
 
 End PTSet.
