backend/AliasLib.v
@@ -1,0 +1,60 @@
+Require String.
+
+Open Scope string_scope.
+
+Ltac move_to_top x :=
+  match reverse goal with
+  | H : _ |- _ => try move x after H
+  end.
+
+Tactic Notation "assert_eq" ident(x) constr(v) :=
+  let H := fresh in
+  assert (x = v) as H by reflexivity;
+  clear H.
+
+Tactic Notation "Case_aux" ident(x) constr(name) :=
+  first [
+    set (x := name); move_to_top x
+  | assert_eq x name; move_to_top x
+  | fail 1 "because we are working on a different case" ].
+Tactic Notation "Case" constr(name) := Case_aux Case name.
+Tactic Notation "SCase" constr(name) := Case_aux SCase name.
+Tactic Notation "SSCase" constr(name) := Case_aux SSCase name.
+Tactic Notation "SSSCase" constr(name) := Case_aux SSSCase name.
+Tactic Notation "SSSSCase" constr(name) := Case_aux SSSSCase name.
+Tactic Notation "SSSSSCase" constr(name) := Case_aux SSSSSCase name.
+Tactic Notation "SSSSSSCase" constr(name) := Case_aux SSSSSSCase name.
+Tactic Notation "SSSSSSSCase" constr(name) := Case_aux SSSSSSSCase name.
+Tactic Notation "SSSSSSSSCase" constr(name) := Case_aux SSSSSSSSCase name.
+Tactic Notation "SSSSSSSSSCase" constr(name) := Case_aux SSSSSSSSSCase name.
+
+Ltac unalias := repeat (autounfold with unalias in *).
+
+Ltac feed H :=
+  match type of H with
+  | ?foo -> _ =>
+    let FOO := fresh in
+    assert foo as FOO; [|specialize (H FOO); clear FOO]
+  end.
+
+Ltac feed_all H := feed H; [|try feed_all H].
+
+Ltac feed_n n H :=
+  match constr:n with
+  | O => idtac
+  | (S ?m) => feed H ; [| feed_n m H]
+  end.
+
+Ltac notHyp P :=
+  match goal with
+  | [ _ : P |- _ ] => fail 1
+  | _ =>
+    match P with
+    | ?P1 /\ ?P2 => first [ notHyp P1 | notHyp P2 | fail 2 ]
+    | _ => idtac
+    end
+  end.
+
+Ltac extend pf :=
+  let t := type of pf in
+  notHyp t; pose proof pf.
