backend/AliasSoundness.v
@@ -1,0 +1,1613 @@
+Require Import BinInt.
+
+Require Import AST.
+Require Import Coqlib.
+Require Import Globalenvs.
+Require Import Integers.
+Require Import Kildall.
+Require Import Maps.
+Require Import Memory.
+Require Import Op.
+Require Import Registers.
+Require Import RTL.
+Require Import Values.
+
+Require Import AliasAbstract.
+Require Import AliasLib.
+Require Import AliasMemMap.
+Require Import AliasPTSet.
+Require Import AliasRegMap.
+Require Import AliasSolver.
+Require Import AliasTransfer.
+
+Definition abstracter := block -> option ablock.
+
+Definition valsat (v: val) (abs: abstracter) (s: PTSet.t) :=
+  match v with
+  | Vptr b o =>
+    match abs b with
+    | Some ab => PTSet.In (Loc ab o) s
+    | None    => PTSet.ge s PTSet.top
+    end
+  | _        => True
+  end.
+Hint Unfold valsat: unalias.
+
+Definition regsat (r: reg) (rs: regset) (abs: abstracter) (rmap: RegMap.t) :=
+  valsat rs#r abs (RegMap.get r rmap).
+Hint Unfold regsat: unalias.
+
+Definition memsat
+  (b: block) (o: Int.int) (m: mem) (abs: abstracter) (mmap: MemMap.t)
+  :=
+  forall v
+    (LOAD: Mem.loadv Mint32 m (Vptr b o) = Some v)
+    ,
+    (match abs b with
+     | Some ab => valsat v abs (MemMap.get (Loc ab o) mmap)
+     | None    => False
+     end).
+Hint Unfold memsat: unalias.
+
+Definition ok_abs_mem (abs: abstracter) (m: mem) :=
+  forall b, abs b <> None <-> Mem.valid_block m b.
+Hint Unfold ok_abs_mem : unalias.
+
+Definition ok_abs_genv (abs: abstracter) (ge: genv) :=
+  forall i b
+    (FIND: Genv.find_symbol ge i = Some b)
+    ,
+    abs b = Some (Global i).
+Hint Unfold ok_abs_genv : unalias.
+
+(* This is factored out to delay the instantiation of rmap, mmap in ok_stack *)
+Inductive ok_abs_result_stack f pc rs rret abs: Prop :=
+| ok_abs_result_stack_intro: forall rmap mmap
+  (RPC:  (analysis f)#pc = (rmap, mmap))
+  (RSAT: forall r, regsat r rs abs rmap)
+  (RET:  PTSet.ge (RegMap.get rret rmap) PTSet.top) (* same as eq, easier *)
+  (MTOP: MemMap.ge mmap MemMap.top)
+  ,
+  ok_abs_result_stack f pc rs rret abs.
+
+Inductive ok_stack (ge: genv) (b: block): list stackframe -> Prop :=
+| ok_stack_nil:
+  ok_stack ge b nil
+| ok_stack_cons: forall r f bsp pc rs stk abs
+  (STK:  ok_stack ge b stk)
+  (MEM:  forall b', abs b' <> None -> (b' < b)%Z)
+  (GENV: ok_abs_genv abs ge)
+  (SP:   abs bsp = Some Stack)
+  (RES:  ok_abs_result_stack f pc rs r abs)
+  ,
+  ok_stack ge b (Stackframe r f (Vptr bsp Int.zero) pc rs :: stk)
+.
+
+(* This is factored out to delay the instantiation of rmap, mmap in satisfy *)
+Inductive ok_abs_result f pc rs m abs: Prop :=
+| ok_abs_result_intro: forall rmap mmap
+  (RPC:  (analysis f)#pc = (rmap, mmap))
+  (RSAT: forall r, regsat r rs abs rmap)
+  (MSAT: forall b o, memsat b o m abs mmap)
+  ,
+  ok_abs_result f pc rs m abs.
+
+Inductive satisfy (ge: genv) (abs: abstracter): state -> Prop :=
+| satisfy_state: forall cs f bsp pc rs m
+  (STK:  ok_stack ge (Mem.nextblock m) cs)
+  (MEM:  ok_abs_mem abs m)
+  (GENV: ok_abs_genv abs ge)
+  (SP:   abs bsp = Some Stack)
+  (RES:  ok_abs_result f pc rs m abs)
+  ,
+  satisfy ge abs (State cs f (Vptr bsp Int.zero) pc rs m)
+| satisfy_callstate: forall cs f args m
+  (MEM:  ok_abs_mem abs m)
+  (STK:  ok_stack ge (Mem.nextblock m) cs)
+  (GENV: ok_abs_genv abs ge)
+  ,
+  satisfy ge abs (Callstate cs f args m)
+| satisfy_returnstate: forall cs v m
+  (MEM:  ok_abs_mem abs m)
+  (STK:  ok_stack ge (Mem.nextblock m) cs)
+  (GENV: ok_abs_genv abs ge)
+  ,
+  satisfy ge abs (Returnstate cs v m)
+.
+
+Lemma regsat_ge1:
+  forall rs rmap abs rmap' r
+    (RSAT: regsat r rs abs rmap)
+    (GE:   RegMap.ge rmap' rmap)
+    ,
+    regsat r rs abs rmap'.
+Proof.
+  intros. unalias. destruct (rs#r); auto. destruct (abs b).
+  now apply GE. eapply PTSet.ge_trans; eauto.
+Qed.
+
+Lemma regsat_ge:
+  forall rs rmap abs rmap'
+    (RSAT: forall r, regsat r rs abs rmap)
+    (GE:   RegMap.ge rmap' rmap)
+    ,
+    (forall r, regsat r rs abs rmap').
+Proof.
+  intros. eapply regsat_ge1; eauto.
+Qed.
+
+Lemma memsat_ge:
+  forall m abs mmap mmap'
+    (MSAT: forall b o, memsat b o m abs mmap)
+    (GE:   MemMap.ge mmap' mmap)
+    ,
+    (forall b o, memsat b o m abs mmap').
+Proof.
+  repeat intro. unalias. specialize (MSAT _ _ _ LOAD).
+  destruct (abs b), v as [ | | | bv ov]; auto. destruct (abs bv).
+  now apply GE.
+  eapply PTSet.ge_trans; eauto.
+Qed.
+
+Lemma regsat_assign_not_vptr:
+  forall rs rmap abs v rdst
+    (RSAT: forall r, regsat r rs abs rmap)
+    (NPTR: match v with Vptr _ _ => False | _ => True end)
+    ,
+    (forall r, regsat r rs#rdst<-v abs rmap).
+Proof.
+  intros. specialize (RSAT r). unalias.
+  destruct (peq r rdst).
+  subst. rewrite Regmap.gss. destruct v; auto.
+  contradiction.
+  rewrite Regmap.gso; auto.
+Qed.
+
+Lemma regsat_assign_other:
+  forall r res v rmap abs rs
+    (RSAT:  forall r, regsat r rs abs rmap)
+    (OTHER: res <> r)
+    ,
+    regsat r rs#res<-v abs rmap.
+Proof.
+  intros. specialize (RSAT r). unalias. rewrite Regmap.gso; auto.
+Qed.
+
+Lemma regsat_top:
+  forall rs abs,
+    (forall r, regsat r rs abs RegMap.top).
+Proof.
+  intros. unalias. destruct (rs#r) as []_eqn; auto. destruct (abs b) as []_eqn.
+  apply RegMap.get_top. apply PTSet.In_top.
+  apply RegMap.get_top.
+Qed.
+
+Notation alias_interprets ge s := (exists abs, satisfy ge abs s).
+
+Theorem alias_interprets_init:
+  forall p st
+    (IS:   initial_state p st),
+    alias_interprets (Genv.globalenv p) st.
+Proof.
+  intros. inv IS.
+  exists (fun b =>
+    if zlt b (Mem.nextblock m0)
+      then
+        match Genv.invert_symbol ge b with
+        | Some i => Some (Global i)
+        | None   => Some Other
+        end
+      else None
+  ).
+  constructor.
+  Case "ok_abs_mem".
+  split; intros; destruct (zlt b0 (Mem.nextblock m0)); auto. congruence.
+  destruct (Genv.invert_symbol); congruence.
+  Case "ok_stack".
+  constructor.
+  Case "ok_abs_genv".
+  unalias; intros. destruct (zlt b0 (Mem.nextblock m0)).
+  eapply Genv.find_invert_symbol in FIND. unfold ge. now rewrite FIND.
+  eapply Genv.find_symbol_not_fresh in FIND; eauto. contradiction.
+Qed.
+
+Ltac regsat_intro_unsafe rs r :=
+  match goal with
+  | H: Vptr _ _ = rs#r |- _ => apply symmetry in H; regsat_intro_unsafe rs r
+  | R: (forall r, regsat r rs _ _),
+    H: rs#r = Vptr _ _ |- _ =>
+      let IN := fresh "IN" in
+      pose proof (R r) as IN; unfold regsat, valsat in IN; rewrite H in IN
+  end.
+Tactic Notation "regsat_intro" constr(rs) constr(r) := regsat_intro_unsafe rs r.
+
+Ltac merge :=
+  match goal with
+  | H: ?x = ?x |- _ => clear H; merge
+  | H: (_, _) = (_, _) |- _ => inv H; merge
+  | H1: ?a = None,
+    H2: ?b = None |- _ => idtac (* prevents a loop *)
+  | H1: ?x = ?a,
+    H2: ?x = ?b |- _ =>
+    rewrite H1 in H2; inv H2; merge
+  | H1: ?a = ?x,
+    H2: ?b = ?x |- _ =>
+    rewrite <- H1 in H2; inv H2; merge
+  | H1: ?x = ?a,
+    H2: ?b = ?x |- _ =>
+    rewrite H1 in H2; inv H2; merge
+  | |- _ => idtac
+  end.
+
+Ltac regsat_tac :=
+  simpl in *;
+  match goal with
+  (* Easy case: same rs, higher rmap *)
+  | H: forall r, regsat r ?rs ?abs ?rmap
+    |- forall r, regsat r ?rs ?abs (RegMap.add _ _ ?rmap) =>
+    eapply regsat_ge; [apply H | apply RegMap.ge_add]
+  (* Simple cases: assigning something that is not a Vptr *)
+  | |- forall r, regsat r _#_<-?v _ _ =>
+    let ok := constr : (
+      match v with (Vundef | Vint _ | Vfloat _) => true | _ => false end
+    ) in
+    match v with
+    | true  => eapply regsat_assign_not_vptr; [ | auto]; regsat_tac
+    | false => fail
+    end
+  | |- forall r, regsat r _#_<-(if ?cond then _ else _) _ _ =>
+    destruct cond as []_eqn; regsat_tac
+  | H: context [if ?cond then _ else _] |- _ =>
+    destruct cond as []_eqn; try solve [inv H]; regsat_tac
+
+  | |- match ?foo with
+       | Vundef => _ | Vint _ => _ | Vfloat _ => _ | Vptr _ _ => _
+       end =>
+    destruct foo as []_eqn; regsat_tac
+
+  | |- context [?rs#?r] =>
+    destruct (rs#r) as []_eqn; simpl; try regsat_intro rs r; regsat_tac
+
+  | H: context [?rs#?r] |- _ =>
+    destruct (rs#r); simpl in H; inv H; try regsat_intro rs r; regsat_tac
+
+  | H: context [match ?rs ## ?args with | nil => _ | _ :: _ => _ end] |- _ =>
+    destruct args; simpl in H; try solve [inv H]; regsat_tac
+
+  | v: val
+    |- forall r, regsat r _#_<-?v _ _ =>
+    destruct v; regsat_tac
+
+  | |- match ?abs ?b with | Some _ => _ | None => _ end =>
+    destruct (abs b) as []_eqn; regsat_tac
+
+  | G: ok_abs_genv _ ?ge,
+    H: Genv.find_symbol ?ge _ = _
+    |- _ =>
+    specialize (G _ _ H); merge; regsat_tac
+
+  (* Almost done *)
+  | |- PTSet.In _ (RegMap.get ?r (RegMap.add ?r _ _)) =>
+    apply RegMap.get_add_same; regsat_tac
+  | |- PTSet.ge (RegMap.get ?r (RegMap.add ?r _ _)) _ =>
+    eapply PTSet.ge_trans; [apply RegMap.get_add_same | auto]; regsat_tac
+
+  | |- forall r, regsat r _#?res<-_ _ _ =>
+    let r := fresh "r" in intro r; destruct (peq res r);
+    [ subst; unfold regsat, valsat; rewrite Regmap.gss
+    | apply regsat_assign_other
+    ];
+    regsat_tac
+(*
+  | c: condition |- _ => destruct c; regsat_tac
+  | c: comparison |- _ => destruct c; regsat_tac
+*)
+  (* Non-recursive cases *)
+  | H: _ = Vptr _ _ |- _ => try solve [inv H]
+  | H: Vptr _ _ = _ |- _ => try solve [inv H]
+
+  | |- _ => auto
+  end.
+
+Ltac crunch_eval :=
+  match goal with
+  | H: Val.of_optbool _ = _ |- _ => unfold Val.of_optbool in H; crunch_eval
+  | H: Val.add _ _ = _ |- _ => unfold Val.add in *; crunch_eval
+  | H: Val.mul _ _ = _ |- _ => unfold Val.mul in *; crunch_eval
+  | H: symbol_address _ _ _ = _ |- _ => unfold symbol_address in *; crunch_eval
+  | H: Vptr _ _ = Vptr _ _ |- _ => inv H; crunch_eval
+  | H: Some _ = None   |- _ => inv H
+  | H: None   = Some _ |- _ => inv H
+  | H: Some _ = Some _ |- _ => inv H; crunch_eval
+  | H: (match _##?args with | nil => _ | _::_ => _ end) = _ |- _ =>
+    destruct args; simpl in H; try solve [inv H]; crunch_eval
+  | H: (match ?rs#?r with
+        | Vundef => _ | Vint _ => _ | Vfloat _ => _ | Vptr _ _ => _
+        end) = _ |- _ =>
+    destruct rs#r as []_eqn; [ | | | regsat_intro rs r]; try solve [inv H]; crunch_eval
+  | H: (if ?cond then _ else _) = _ |- _ =>
+    destruct cond as []_eqn; try solve [inv H]; crunch_eval
+  | H: (match ?opt with | Some _ => _ | None   => _ end) = _ |- _ =>
+    destruct opt as []_eqn; try solve [inv H]; crunch_eval
+  | H: (match ?opt with | Some _ => _ | None => _ end) |- _ =>
+    destruct opt as []_eqn; try solve [congruence]; crunch_eval
+  | H: (match ?val with
+        | Vundef => _ | Vint _ => _ | Vfloat _ => _ | Vptr _ _ => _
+        end) = _ |- _ =>
+    destruct val as []_eqn; try solve [inv H]; crunch_eval
+  | a: addressing |- _          => destruct a; simpl in *; crunch_eval
+  (*| H: offset_sp ?sp _ = _ |- _ => unfold offset_sp in H; crunch_eval*)
+  | H: option_map _ _ = _ |- _  => unfold option_map in H; crunch_eval
+  | _ => idtac
+  end.
+
+Lemma In_unknown_offset:
+  forall b o s
+    (IN: PTSet.In (Loc b o) s)
+    ,
+    (forall o', PTSet.In (Loc b o') (unknown_offset s)).
+Proof.
+  intros. unfold unknown_offset. eapply PTSet.fold_adds_prop; intros; eauto.
+  simpl. apply PTSet.loc_In_add_blk.
+  destruct y; now apply PTSet.In_add.
+Qed.
+
+Theorem In_unknown_offset_same:
+  forall p s
+    (IN: PTSet.In p s),
+    PTSet.In p (unknown_offset s).
+Proof.
+  intros. unfold unknown_offset. eapply PTSet.fold_adds_prop; intros; eauto.
+  destruct p. apply PTSet.In_add_same. apply PTSet.loc_In_add_blk.
+  destruct y; now apply PTSet.In_add.
+Qed.
+
+Lemma unknown_offset_top:
+  forall s
+    (GETOP: PTSet.ge s PTSet.top)
+    ,
+    PTSet.ge (unknown_offset s) PTSet.top.
+Proof.
+  repeat intro. specialize (GETOP _ H). apply In_unknown_offset_same. auto.
+Qed.
+
+Lemma In_shift_offset:
+  forall b o s o' oshift
+    (IN: PTSet.In (Loc b o) s)
+    (SH: o' = Int.add o oshift)
+    ,
+    PTSet.In (Loc b o') (shift_offset s oshift).
+Proof.
+  intros. subst. rewrite Int.add_commut.
+  unfold shift_offset. eapply PTSet.fold_adds_prop; intros; eauto; simpl.
+  apply PTSet.In_add_same.
+  destruct y; now apply PTSet.In_add.
+Qed.
+
+Lemma shift_offset_top:
+  forall s
+    (GETOP: PTSet.ge s PTSet.top)
+    ,
+    (forall oshift, PTSet.ge (shift_offset s oshift) PTSet.top).
+Proof.
+  repeat intro. clear H. unfold shift_offset.
+  apply PTSet.fold_adds_prop with (e := Blk All); intros.
+  apply (GETOP (Blk All)). apply PTSet.In_top.
+  destruct elt; destruct a; try solve
+  [ apply PTSet.In_add_lt; simpl; now intuition
+  | apply PTSet.In_add_same
+  ].
+  destruct y; now apply PTSet.In_add.
+Qed.
+
+Lemma load_valid_block:
+  forall chunk m b ofs v,
+    Mem.load chunk m b ofs = Some v ->
+    Mem.valid_block m b.
+Proof.
+  intros. eapply Mem.load_valid_access in H. eapply Mem.valid_access_implies in H.
+  eapply Mem.valid_access_valid_block in H. auto. constructor.
+Qed.
+
+Lemma memsat_top:
+  forall m abs
+    (OKAM: ok_abs_mem abs m)
+    ,
+    (forall b o, memsat b o m abs MemMap.top).
+Proof.
+  unalias. intros. destruct (abs b) as []_eqn.
+  destruct v; auto. destruct (abs b0) as []_eqn.
+  apply MemMap.get_top. apply PTSet.In_top.
+  apply MemMap.get_top.
+  simpl in LOAD. apply load_valid_block in LOAD. now apply OKAM in LOAD.
+Qed.
+
+Lemma memsat_free:
+  forall m abs ptm bf lo hi m'
+    (MSAT: forall b o, memsat b o m abs ptm)
+    (FREE: Mem.free m bf lo hi = Some m')
+    ,
+    (forall b o, memsat b o m' abs ptm).
+Proof.
+  intros. unfold memsat, valsat in *. intros. specialize (MSAT b o v).
+  feed MSAT. simpl in *. erewrite Mem.load_free in LOAD. eauto. eauto.
+  destruct (zeq b bf); auto. subst. apply Mem.load_valid_access in LOAD.
+  eapply Mem.valid_access_free_inv_2 in LOAD; eauto.
+  auto.
+Qed.
+
+Lemma ok_abs_mem_store:
+  forall abs m chunk b o v m'
+    (OKAM: ok_abs_mem abs m)
+    (STOR: Mem.store chunk m b o v = Some m')
+    ,
+    ok_abs_mem abs m'.
+Proof.
+  unalias. split; intros.
+  eapply Mem.store_valid_block_1; eauto. apply OKAM. auto.
+  apply OKAM. eapply Mem.store_valid_block_2; eauto.
+Qed.
+
+Lemma ok_abs_mem_free:
+  forall abs m b o s m'
+    (OKAM: ok_abs_mem abs m)
+    (FREE: Mem.free m b o s = Some m')
+    ,
+    ok_abs_mem abs m'.
+Proof.
+  unalias. split; intros.
+  eapply Mem.valid_block_free_1; eauto. apply OKAM. auto.
+  apply OKAM. eapply Mem.valid_block_free_2; eauto.
+Qed.
+
+Lemma ok_abs_mem_storebytes:
+  forall abs m b o s m'
+    (OK: ok_abs_mem abs m)
+    (SB: Mem.storebytes m b o s = Some m')
+    ,
+    ok_abs_mem abs m'.
+Proof.
+  unalias; intros. specialize (OK b0). split; intros. apply OK in H.
+  eapply Mem.storebytes_valid_block_1; eauto. apply OK.
+  eapply Mem.storebytes_valid_block_2; eauto.
+Qed.
+
+Lemma ok_stack_incr:
+  forall stk ge b, ok_stack ge b stk -> forall b', b <= b' -> ok_stack ge b' stk.
+Proof.
+  induction 1; intros; econstructor; eauto. intros. specialize (MEM b'0 H1). omega.
+Qed.
+
+Lemma ok_stack_alloc:
+  forall stack ge m m' lo hi b,
+    ok_stack ge (Mem.nextblock m) stack ->
+    Mem.alloc m lo hi = (m', b) ->
+    ok_stack ge (Mem.nextblock m') stack.
+Proof.
+  intros. eapply ok_stack_incr; eauto.
+  setoid_rewrite Mem.nextblock_alloc at 2; eauto. omega.
+Qed.
+
+Lemma load_alloc_other':
+  forall m1 lo hi m2 b,
+    Mem.alloc m1 lo hi = (m2, b) ->
+    forall b' ofs chunk,
+    b <> b' ->
+    Mem.load chunk m2 b' ofs = Mem.load chunk m1 b' ofs.
+Proof.
+  intros. destruct (Mem.load chunk m1 b' ofs) as []_eqn. pose proof Heqo as L.
+  eapply Mem.load_valid_access in Heqo. eapply Mem.valid_access_implies in Heqo.
+  eapply Mem.valid_access_valid_block in Heqo. erewrite Mem.load_alloc_unchanged; eauto.
+  constructor. destruct (Mem.load chunk m2 b' ofs) as []_eqn; auto.
+  eapply Mem.load_valid_access in Heqo0. eapply Mem.valid_access_implies in Heqo0.
+  eapply Mem.valid_access_alloc_inv in Heqo0; eauto. destruct (eq_block b' b).
+  congruence. eapply Mem.valid_access_load in Heqo0. destruct Heqo0. congruence.
+  constructor.
+Qed.
+
+Lemma load_vptr_Mint32:
+  forall chunk m a b o
+    (LOAD: Mem.loadv chunk m a = Some (Vptr b o))
+    ,
+    chunk = Mint32.
+Proof.
+  intros. unfold Mem.loadv in LOAD. destruct a; try solve [inv LOAD].
+  apply Mem.load_result in LOAD. symmetry in LOAD. apply decode_val_pointer_inv in LOAD.
+  destruct LOAD. subst. auto.
+Qed.
+
+Lemma In_image_of_ptset:
+  forall x y mmap s,
+    PTSet.In x s ->
+    PTSet.In y (MemMap.get x mmap) ->
+    PTSet.In y (image_of_ptset s mmap).
+Proof.
+  intros. unfold image_of_ptset. eapply PTSet.fold_adds_prop; eauto; intros.
+  now apply PTSet.ge_join_l.
+  now apply PTSet.ge_join_r.
+Qed.
+
+Lemma In_add_ptset_to_image:
+  forall x y sfrom sto mmap
+    (FROM: PTSet.In x sfrom)
+    (TO:   PTSet.In y sto)
+    ,
+    PTSet.In x (MemMap.get y (add_ptset_to_image sfrom sto mmap)).
+Proof.
+  intros. unfold add_ptset_to_image. eapply PTSet.fold_adds_prop; eauto; intros.
+  now apply MemMap.get_add_same.
+  now apply MemMap.ge_add.
+Qed.
+
+Lemma ge_add_ptset_to_image:
+  forall mmap s s',
+    MemMap.ge (add_ptset_to_image s s' mmap) mmap.
+Proof.
+  intros. unfold add_ptset_to_image. apply PTSet.fold_preserves_prop; intros.
+  apply MemMap.ge_refl.
+  eapply MemMap.ge_trans; eauto. apply MemMap.ge_add.
+Qed.
+
+Lemma addr_image_correct:
+  forall ge rs rmap abs addr args b o ab s bsp
+    (GENV: ok_abs_genv abs ge)
+    (SP: abs bsp = Some Stack)
+    (RSAT: forall r, regsat r rs abs rmap)
+    (EA: eval_addressing ge (Vptr bsp Int.zero) addr rs##args = Some (Vptr b o))
+    (ABS: abs b = Some ab)
+    (MPTA: addr_image addr args rmap = Some s)
+    ,
+    PTSet.In (Loc ab o) s.
+Proof.
+  intros.
+  crunch_eval; merge.
+  eapply In_shift_offset; eauto.
+  apply PTSet.ge_join_r. eapply In_unknown_offset; eauto.
+  apply PTSet.ge_join_l. eapply In_unknown_offset; eauto.
+  eapply In_unknown_offset; eauto.
+  specialize (GENV _ _ Heqo0). merge. apply PTSet.In_singleton.
+  specialize (GENV _ _ Heqo). merge. apply PTSet.loc_In_add_blk.
+  specialize (GENV _ _ Heqo0). merge. apply PTSet.loc_In_add_blk.
+  rewrite Int.add_zero_l. apply PTSet.In_singleton.
+Qed.
+
+Lemma fold_left_preserves_prop:
+  forall S F (P: S -> Prop) (f: S -> F -> S) l s,
+    P s ->
+    (forall x y, P x -> P (f x y)) ->
+    P (fold_left f l s).
+Proof.
+  induction l; simpl; auto.
+Qed.
+
+Lemma fold_left_adds_prop:
+  forall E S (e: E) (P: S -> Prop) (f: S -> E -> S) l s0,
+    In e l ->
+    (forall x, P (f x e)) ->
+    (forall x y, P x -> P (f x y)) ->
+    P (fold_left f l s0).
+Proof.
+  induction l; intros.
+  inversion H.
+  inversion_clear H. subst.
+  simpl. apply fold_left_preserves_prop; auto.
+  eapply IHl; eauto.
+Qed.
+
+Theorem alias_interprets_step:
+  forall ge st t st'
+    (AI:   alias_interprets ge st)
+    (STEP: step ge st t st')
+    ,
+    alias_interprets ge st'.
+Proof.
+  intros. destruct AI as [abs SAT].
+  destruct st; destruct st'; try solve [inv STEP]; inv SAT; try inv RES.
+
+  Case "State -> State".
+  unfold analysis in RPC. destruct (failure_prone_analysis f) as [res|]_eqn.
+  SCase "Kildall terminated".
+  pose proof Heqo as FPS.
+  eapply Solver.fixpoint_solution with (n:=pc)(s:=pc0) in FPS;
+  [ |
+  unfold successors; unfold successors_list; rewrite PTree.gmap1;
+  inv STEP; rewrite H6; simpl; try destruct b; auto; eapply list_nth_z_in; eauto
+  ].
+  rewrite RPC in FPS. unfold Solver.L.ge in FPS.
+  destruct (res#pc0) as [rmap'' mmap'']_eqn.
+  destruct (transf (fn_code f) pc (rmap, mmap)) as [rmap' mmap']_eqn.
+  destruct FPS as [RGE MGE].
+  inv STEP;
+  match goal with A : ?f ! ?pc = _, B : transf ?f ?pc _ = _ |- _ =>
+    unfold transf in B; rewrite A in B; inv B
+  end;
+  try solve [
+    exists abs; constructor; auto; econstructor;
+    [ unfold analysis; rewrite Heqo; apply Heqt0
+    | eapply regsat_ge; eauto | eapply memsat_ge; eauto]
+  ].
+
+  SSCase "Iop".
+  exists abs; constructor; auto.
+  SSSCase "ok_abs_result".
+  econstructor.
+  SSSSCase "result".
+  unfold analysis. rewrite Heqo. eauto.
+  SSSSCase "regsat".
+  eapply regsat_ge; eauto.
+
+  destruct op; simpl in *; repeat (crunch_eval; regsat_tac).
+  SSSSSCase "Oindirectsymbol".
+  apply PTSet.In_singleton.
+  SSSSSCase "Osub".
+  eapply In_unknown_offset; eauto.
+  apply unknown_offset_top; auto.
+  SSSSSCase "Olea Aindexed".
+  eapply In_shift_offset; eauto.
+  apply shift_offset_top; auto.
+  SSSSSCase "Olea Aindexed2".
+  apply PTSet.ge_join_r. eapply In_unknown_offset; eauto.
+  eapply PTSet.ge_trans. apply PTSet.ge_join_r. apply unknown_offset_top; auto.
+  apply PTSet.ge_join_l. eapply In_unknown_offset; eauto.
+  eapply PTSet.ge_trans. apply PTSet.ge_join_l. apply unknown_offset_top; auto.
+  SSSSSCase "Olea Aindexed2scaled".
+  eapply In_unknown_offset; eauto.
+  apply unknown_offset_top; auto.
+  SSSSSCase "Olea Aglobal".
+  apply PTSet.In_singleton.
+  SSSSSCase "Olea Abased".
+  apply PTSet.loc_In_add_blk.
+  SSSSSCase "Olea Abasedscaled".
+  apply PTSet.loc_In_add_blk.
+  SSSSSCase "Olea Ainstack".
+  rewrite Int.add_zero_l. apply PTSet.In_singleton.
+  SSSSCase "memsat".
+  eapply memsat_ge; eauto.
+  SSCase "Iload".
+  exists abs; constructor; auto.
+  SSSCase "ok_abs_result".
+  econstructor.
+  SSSSCase "result".
+  unfold analysis. rewrite Heqo. eauto.
+  SSSSCase "regsat".
+  eapply regsat_ge; eauto.
+  destruct chunk; try solve [inv H0;
+    eapply regsat_assign_not_vptr;
+      [ eapply regsat_ge; [auto | apply RegMap.ge_add]
+      | destruct v; auto; apply load_vptr_Mint32 in H14; congruence
+      ]
+  ].
+  intros. destruct (peq dst r).
+  SSSSSCase "r = dst".
+  subst. unfold regsat, valsat. rewrite Regmap.gss. destruct v; auto.
+  destruct a as [ | | |ba oa]; try solve [inv H14].
+  specialize (MSAT _ _ _ H14).
+  destruct (abs ba) as []_eqn; [|contradiction].
+  destruct (abs b) as []_eqn.
+  SSSSSSCase "abs b = Some".
+  crunch_eval; inv H0; apply RegMap.get_add_same; eapply In_image_of_ptset;
+    eauto; merge.
+  eapply In_shift_offset; eauto.
+  apply PTSet.ge_join_r. eapply In_unknown_offset; eauto.
+  apply PTSet.ge_join_l. eapply In_unknown_offset; eauto.
+  eapply In_unknown_offset; eauto.
+  specialize (GENV _ _ Heqo2). merge. apply PTSet.In_singleton.
+  specialize (GENV _ _ Heqo1). merge. apply PTSet.loc_In_add_blk.
+  specialize (GENV _ _ Heqo1). merge. apply PTSet.loc_In_add_blk.
+  rewrite Int.add_zero_l. apply PTSet.In_singleton.
+  SSSSSSCase "abs b = None".
+  crunch_eval; inv H0; (
+  eapply PTSet.ge_trans;
+    [ apply RegMap.get_add_same
+    | repeat intro; eapply In_image_of_ptset; [ | apply MSAT; apply PTSet.In_top]
+    ]); merge.
+  eapply In_shift_offset; eauto.
+  apply PTSet.ge_join_r. eapply In_unknown_offset; eauto.
+  apply PTSet.ge_join_l. eapply In_unknown_offset; eauto.
+  eapply In_unknown_offset; eauto.
+  apply unknown_offset_top; auto. apply PTSet.In_top.
+  specialize (GENV _ _ Heqo2). merge. apply PTSet.In_singleton.
+  specialize (GENV _ _ Heqo3). merge. apply PTSet.loc_In_add_blk.
+  specialize (GENV _ _ Heqo3). merge. apply PTSet.loc_In_add_blk.
+  merge. rewrite Int.add_zero_l. apply PTSet.In_singleton.
+  SSSSSCase "r <> dst".
+  eapply regsat_assign_other; eauto. destruct addr_image; inv H0; auto.
+  eapply regsat_ge; eauto. apply RegMap.ge_add.
+  SSSSCase "memsat".
+  eapply memsat_ge; eauto. eapply MemMap.ge_trans; eauto.
+  destruct chunk; try solve [inv H0; apply MemMap.ge_refl].
+  destruct addr_image; inv H0; apply MemMap.ge_refl.
+  SSCase "Istore".
+  assert (MGE': MemMap.ge mmap' mmap) by (
+  destruct chunk; try solve [inv H0; apply MemMap.ge_refl];
+  destruct addr_image; inv H0;
+    [ apply ge_add_ptset_to_image
+    | apply MemMap.ge_refl
+    ]).
+  exists abs. destruct a; try solve [inv H14]. constructor; auto.
+  SSSCase "ok_stack".
+  erewrite Mem.nextblock_store; eauto.
+  SSSCase "ok_abs_mem".
+  eapply ok_abs_mem_store; eauto.
+  SSSCase "ok_abs_result".
+  econstructor.
+  SSSSCase "result".
+  unfold analysis. rewrite Heqo. eauto.
+  SSSSCase "regsat".
+  eapply regsat_ge; eauto. eapply RegMap.ge_trans; eauto.
+  destruct chunk; try solve [inv H0; apply RegMap.ge_refl].
+  destruct addr_image; inv H0; apply RegMap.ge_refl.
+  SSSSCase "memsat".
+  eapply memsat_ge; eauto.
+  intros. specialize (MSAT b0 o). unfold memsat, valsat in *. intros.
+  pose proof (Mem.valid_access_load m Mint32 b0 (Int.unsigned o)) as LOAD'.
+  feed LOAD'. eapply Mem.store_valid_access_2; eauto. eapply Mem.load_valid_access; eauto.
+  destruct LOAD' as [v' LOAD']. specialize (MSAT _ LOAD').
+  destruct (zeq b b0).
+  SSSSSCase "Stored in b".
+  subst.
+  destruct (zlt (Int.unsigned i) (Int.unsigned o + size_chunk Mint32)).
+  destruct (zlt (Int.unsigned o) (Int.unsigned i + size_chunk chunk)).
+  SSSSSSCase "Overlapped offset o".
+  destruct (abs b0) as []_eqn; [|contradiction].
+  destruct v; auto. pose proof LOAD as LOAD''.
+  eapply Mem.load_pointer_store in LOAD; eauto.
+  intuition; try solve [omegaContradiction]. subst. simpl in *.
+  assert (i = o)
+    by (apply f_equal with (f:=Int.repr) in H5; rewrite Int.repr_unsigned in H5;
+      rewrite Int.repr_unsigned in H5; auto). subst. clear z z0 H5.
+  regsat_intro rs0 src.
+  destruct (addr_image addr args rmap) as []_eqn; [|crunch_eval]. inv H0.
+  eapply addr_image_correct in Heqo1; eauto.
+  destruct (abs b) as []_eqn.
+  SSSSSSSSCase "abs b = Some".
+  apply In_add_ptset_to_image; auto.
+  SSSSSSSSCase "abs b = None".
+  repeat intro. apply In_add_ptset_to_image; auto.
+  SSSSSSCase "Didn't overlap offset o".
+  simpl in LOAD.
+  erewrite Mem.load_store_other in LOAD; eauto; [|right; right; omega]. merge.
+  destruct (abs b0) as []_eqn; [|contradiction].
+  destruct v; auto.
+  destruct (abs b) as []_eqn.
+  SSSSSSSCase "abs b = Some".
+  now apply MGE'.
+  SSSSSSSCase "abs b = None".
+  eapply PTSet.ge_trans; eauto.
+  SSSSSSCase "Didn't overlap offset o, for another reason".
+  simpl in LOAD.
+  erewrite Mem.load_store_other in LOAD; eauto; [|right; left; omega]. merge.
+  destruct (abs b0) as []_eqn; [|contradiction].
+  destruct v; auto.
+  destruct (abs b) as []_eqn.
+  SSSSSSSCase "abs b = Some".
+  now apply MGE'.
+  SSSSSSSCase "abs b = None".
+  eapply PTSet.ge_trans; eauto.
+  SSSSSCase "Didn't store in b0".
+  simpl in LOAD. erewrite Mem.load_store_other in LOAD; eauto. merge.
+  destruct (abs b0) as []_eqn; [|contradiction].
+  destruct v; auto.
+  destruct (abs b1) as []_eqn.
+  SSSSSSCase "abs b1 = Some".
+  now apply MGE'.
+  SSSSSSCase "abs b1 = None".
+  eapply PTSet.ge_trans; eauto.
+  SSCase "Ibuiltin".
+  assert (RGE': RegMap.ge rmap' rmap) by (
+  destruct ef; repeat (
+    try solve [inv H0; apply RegMap.ge_add];
+    try solve [inv H0; apply RegMap.ge_refl];
+    destruct args)).
+  assert (MGE': MemMap.ge mmap' mmap).
+  destruct ef; repeat (
+    try solve [inv H0; apply ge_add_ptset_to_image];
+    try solve [inv H0; apply MemMap.ge_refl];
+    try solve [inv H0; apply MemMap.ge_add];
+    destruct args).
+  destruct ef; inv H13; merge.
+  SSSCase "EF_external".
+  exists abs. constructor; auto.
+  SSSSCase "ok_abs_result".
+  econstructor.
+  SSSSSCase "result".
+  unfold analysis. rewrite Heqo. eauto.
+  SSSSSCase "regsat".
+  intros; destruct (peq res0 r); [subst | eapply regsat_assign_other; eauto;
+    eapply regsat_ge; [eauto | eapply RegMap.ge_trans; eauto]].
+  unfold regsat, valsat. rewrite Regmap.gss. destruct v; auto.
+  inv H1. specialize (GENV _ _ H4). rewrite GENV.
+  eapply PTSet.ge_trans. apply RegMap.get_ge; apply RGE. apply RegMap.get_add_same.
+  apply PTSet.In_add_lt. simpl. tauto.
+  SSSSSCase "memsat".
+  eapply memsat_ge; eauto.
+  SSSCase "EF_builtin".
+  exists abs. constructor; auto.
+  SSSSCase "ok_abs_result".
+  econstructor.
+  SSSSSCase "result".
+  unfold analysis. rewrite Heqo. eauto.
+  SSSSSCase "regsat".
+  intros; destruct (peq res0 r); [subst | eapply regsat_assign_other; eauto;
+    eapply regsat_ge; [eauto | eapply RegMap.ge_trans; eauto]].
+  unfold regsat, valsat. rewrite Regmap.gss. destruct v; auto.
+  inv H1. specialize (GENV _ _ H4). rewrite GENV.
+  eapply PTSet.ge_trans. apply RegMap.get_ge; apply RGE. apply RegMap.get_add_same.
+  apply PTSet.In_add_lt. simpl. tauto.
+  SSSSSCase "memsat".
+  eapply memsat_ge; eauto.
+  SSSCase "EF_vload".
+  exists abs. constructor; auto.
+  SSSSCase "ok_abs_result".
+  econstructor.
+  SSSSSCase "result".
+  unfold analysis. rewrite Heqo. eauto.
+  SSSSSCase "regsat".
+  intros; destruct (peq res0 r); [subst | eapply regsat_assign_other; eauto;
+    eapply regsat_ge; [eauto | eapply RegMap.ge_trans; eauto]].
+  unfold regsat, valsat. rewrite Regmap.gss. destruct v; simpl; auto.
+  regsat_tac.
+  eapply RegMap.get_ge. eauto. apply RegMap.get_add_same. apply PTSet.In_top.
+  eapply PTSet.ge_trans. apply RegMap.get_ge. eauto. apply RegMap.get_add_same.
+  SSSSSCase "memsat".
+  eapply memsat_ge; eauto.
+  inv H1. (* Check whether the store is volatile *)
+  SSSCase "EF_vstore (volatile)".
+  exists abs. constructor; auto.
+  SSSSCase "ok_abs_result".
+  econstructor.
+  SSSSSCase "result".
+  unfold analysis. rewrite Heqo. eauto.
+  SSSSSCase "regsat".
+  intros; destruct (peq res0 r); [subst | eapply regsat_assign_other; eauto;
+    eapply regsat_ge; [eauto | eapply RegMap.ge_trans; eauto]].
+  unfold regsat, valsat. rewrite Regmap.gss. auto.
+  SSSSSCase "memsat".
+  eapply memsat_ge; eauto. eapply MemMap.ge_trans; eauto.
+  SSSCase "EF_vstore (not volatile)".
+  exists abs. constructor; auto.
+  SSSSCase "ok_stack".
+  erewrite Mem.nextblock_store; eauto.
+  SSSSCase "ok_abs_mem".
+  eapply ok_abs_mem_store; eauto.
+  SSSSCase "ok_abs_result".
+  econstructor.
+  SSSSSCase "result".
+  unfold analysis. rewrite Heqo. eauto.
+  SSSSSCase "regsat".
+  intros; destruct (peq res0 r); [subst | eapply regsat_assign_other; eauto;
+    eapply regsat_ge; [eauto | eapply RegMap.ge_trans; eauto]].
+  unfold regsat, valsat. rewrite Regmap.gss. auto.
+  SSSSSCase "memsat".
+  eapply memsat_ge; eauto.
+  repeat (destruct args; try solve [inv H]). inv H. inv H0.
+  intros. specialize (MSAT b0 o). unfold memsat, valsat in *. intros.
+  pose proof (Mem.valid_access_load m Mint32 b0 (Int.unsigned o)) as LOAD'.
+  feed LOAD'. eapply Mem.store_valid_access_2; eauto. eapply Mem.load_valid_access; eauto.
+  destruct LOAD' as [v' LOAD']. specialize (MSAT _ LOAD').
+  destruct (zeq b b0).
+  SSSSSSCase "Stored in b".
+  subst.
+  destruct (zlt (Int.unsigned ofs) (Int.unsigned o + size_chunk Mint32)).
+  destruct (zlt (Int.unsigned o) (Int.unsigned ofs + size_chunk chunk)).
+  SSSSSSSCase "Overlapped offset o".
+  destruct (abs b0) as []_eqn; [|contradiction].
+  destruct v; auto. pose proof LOAD as LOAD''.
+  eapply Mem.load_pointer_store in LOAD; eauto.
+  intuition; try solve [omegaContradiction]. merge. subst. simpl in *.
+  assert (o = ofs)
+    by (apply f_equal with (f:=Int.repr) in H8; rewrite Int.repr_unsigned in H8;
+      rewrite Int.repr_unsigned in H8; auto). subst. clear z z0 H8.
+  regsat_intro rs r0. regsat_intro rs r. rewrite Heqo0 in IN0.
+  destruct (abs b) as []_eqn.
+  SSSSSSSSCase "abs b = Some".
+  apply In_add_ptset_to_image; auto.
+  SSSSSSSSCase "abs b = None".
+  eapply PTSet.ge_trans. repeat intro. apply In_add_ptset_to_image; auto.
+  apply H0. easy.
+  SSSSSSSCase "Didn't overlap offset o".
+  simpl in LOAD.
+  erewrite Mem.load_store_other in LOAD; eauto; [|right; right; omega]. merge.
+  destruct (abs b0) as []_eqn; [|contradiction].
+  destruct v; auto.
+  destruct (abs b) as []_eqn.
+  SSSSSSSSCase "abs b = Some".
+  now apply MGE'.
+  SSSSSSSSCase "abs b = None".
+  eapply PTSet.ge_trans; eauto.
+  SSSSSSSCase "Didn't overlap offset o, for another reason".
+  simpl in LOAD.
+  erewrite Mem.load_store_other in LOAD; eauto; [|right; left; omega]. merge.
+  destruct (abs b0) as []_eqn; [|contradiction].
+  destruct v; auto.
+  destruct (abs b) as []_eqn.
+  SSSSSSSSCase "abs b = Some".
+  now apply MGE'.
+  SSSSSSSSCase "abs b = None".
+  eapply PTSet.ge_trans; eauto.
+  SSSSSSCase "Didn't store in b0".
+  simpl in LOAD. erewrite Mem.load_store_other in LOAD; eauto. merge.
+  destruct (abs b0) as []_eqn; [|contradiction].
+  destruct v; auto.
+  destruct (abs b1) as []_eqn.
+  SSSSSSSCase "abs b1 = Some".
+  now apply MGE'.
+  SSSSSSSCase "abs b1 = None".
+  eapply PTSet.ge_trans; eauto.
+  SSSCase "EF_vload_global".
+  exists abs. constructor; auto.
+  SSSSCase "ok_abs_result".
+  econstructor.
+  SSSSSCase "result".
+  unfold analysis. rewrite Heqo. eauto.
+  SSSSSCase "regsat".
+  intros; destruct (peq res0 r); [subst | eapply regsat_assign_other; eauto;
+    eapply regsat_ge; [eauto | eapply RegMap.ge_trans; eauto]].
+  unfold regsat, valsat. rewrite Regmap.gss. destruct v; auto.
+  regsat_tac.
+  eapply RegMap.get_ge. eauto. apply RegMap.get_add_same. apply PTSet.In_top.
+  eapply PTSet.ge_trans. apply RegMap.get_ge. eauto. apply RegMap.get_add_same.
+  SSSSSCase "memsat".
+  eapply memsat_ge; eauto.
+  inv H2. (* Check whether the store is volatile *)
+  SSSCase "EF_vstore_global (volatile)".
+  exists abs. constructor; auto.
+  SSSSCase "ok_abs_result".
+  econstructor.
+  SSSSSCase "result".
+  unfold analysis. rewrite Heqo. eauto.
+  SSSSSCase "regsat".
+  intros; destruct (peq res0 r); [subst | eapply regsat_assign_other; eauto;
+    eapply regsat_ge; [eauto | eapply RegMap.ge_trans; eauto]].
+  unfold regsat, valsat. rewrite Regmap.gss. auto.
+  SSSSSCase "memsat".
+  eapply memsat_ge; eauto. eapply MemMap.ge_trans; eauto.
+  SSSCase "EF_vstore (not volatile)".
+  exists abs. constructor; auto.
+  SSSSCase "ok_stack".
+  erewrite Mem.nextblock_store; eauto.
+  SSSSCase "ok_abs_mem".
+  eapply ok_abs_mem_store; eauto.
+  SSSSCase "ok_abs_result".
+  econstructor.
+  SSSSSCase "result".
+  unfold analysis. rewrite Heqo. eauto.
+  SSSSSCase "regsat".
+  intros; destruct (peq res0 r); [subst | eapply regsat_assign_other; eauto;
+    eapply regsat_ge; [eauto | eapply RegMap.ge_trans; eauto]].
+  unfold regsat, valsat. rewrite Regmap.gss. auto.
+  SSSSSCase "memsat".
+  specialize (GENV _ _ H1).
+  eapply memsat_ge; eauto.
+  repeat (destruct args; try solve [inv H]). inv H. inv H0.
+  intros b0 o. specialize (MSAT b0 o). unfold memsat, valsat in *.
+  intros v LOAD.
+  pose proof (Mem.valid_access_load m Mint32 b0 (Int.unsigned o)) as LOAD'.
+  feed LOAD'.
+  eapply Mem.store_valid_access_2; eauto.
+  eapply Mem.load_valid_access; eauto.
+  destruct LOAD' as [v' LOAD']. specialize (MSAT _ LOAD').
+  destruct (zeq b b0).
+  SSSSSSCase "Stored in b".
+  subst. rewrite GENV. rewrite GENV in MSAT. destruct v; auto.
+  destruct (zlt (Int.unsigned ofs) (Int.unsigned o + size_chunk Mint32)).
+  destruct (zlt (Int.unsigned o) (Int.unsigned ofs + size_chunk chunk)).
+  SSSSSSSCase "Overlapped offset o".
+  pose proof LOAD as LOAD''.
+  eapply Mem.load_pointer_store in LOAD; eauto.
+  intuition; try solve [omegaContradiction]. merge. subst. simpl in *.
+  assert (o = ofs)
+    by (apply f_equal with (f:=Int.repr) in H8; rewrite Int.repr_unsigned in H8;
+      rewrite Int.repr_unsigned in H8; auto). subst. clear z z0 H8.
+  regsat_intro rs r. rewrite H in H4.
+  destruct (abs b) as []_eqn.
+  SSSSSSSSCase "abs b = Some".
+  apply MemMap.get_add_same. exact IN.
+  SSSSSSSSCase "abs b = None".
+  eapply PTSet.ge_trans. apply MemMap.get_add_same. easy.
+  SSSSSSSCase "Didn't overlap offset o".
+  simpl in LOAD.
+  erewrite Mem.load_store_other in LOAD; eauto; [|right; right; omega]. merge.
+  destruct (abs b) as []_eqn.
+  SSSSSSSSCase "abs b = Some".
+  now apply MGE'.
+  SSSSSSSSCase "abs b = None".
+  eapply PTSet.ge_trans; eauto.
+  SSSSSSSCase "Didn't overlap offset o, for another reason".
+  simpl in LOAD.
+  erewrite Mem.load_store_other in LOAD; eauto; [|right; left; omega]. merge.
+  destruct (abs b) as []_eqn.
+  SSSSSSSSCase "abs b = Some".
+  now apply MGE'.
+  SSSSSSSSCase "abs b = None".
+  eapply PTSet.ge_trans; eauto.
+  SSSSSSCase "Didn't store in b0".
+  simpl in LOAD. erewrite Mem.load_store_other in LOAD; eauto. merge.
+  destruct (abs b0) as []_eqn; [|contradiction].
+  destruct v; auto.
+  destruct (abs b1) as []_eqn.
+  SSSSSSSCase "abs b1 = Some".
+  now apply MGE'.
+  SSSSSSSCase "abs b1 = None".
+  eapply PTSet.ge_trans; eauto.
+  SSSCase "EF_malloc".
+  exists (fun x => if zeq x b then Some (Alloc pc) else abs x).
+  constructor; auto.
+  SSSSCase "ok_stack".
+  erewrite Mem.nextblock_store; [|eauto]. eapply ok_stack_alloc; eauto.
+  SSSSCase "ok_abs_mem".
+  unalias. split; intros.
+  destruct (zeq b0 b); [subst|].
+  eapply Mem.store_valid_block_1; eauto. eapply Mem.valid_new_block; eauto.
+  eapply Mem.store_valid_block_1; eauto. eapply Mem.valid_block_alloc; eauto.
+  apply MEM. auto.
+  destruct (zeq b0 b); [subst|].
+  congruence.
+  apply MEM.
+  eapply Mem.store_valid_block_2 in H2; [|eauto].
+  eapply Mem.valid_block_alloc_inv in H2; [|eauto].
+  inv H2. congruence. auto.
+  SSSSCase "ok_abs_genv".
+  unalias; intros. destruct (zeq b0 b); auto.
+  exfalso. subst. eapply Mem.fresh_block_alloc; eauto. apply MEM.
+  erewrite GENV; [congruence|eauto].
+  SSSSCase "sp".
+  destruct (zeq bsp b); auto.
+  subst. exfalso. eapply Mem.fresh_block_alloc; eauto. apply MEM. congruence.
+  SSSSCase "ok_abs_result".
+  econstructor.
+  SSSSSCase "result".
+  unfold analysis. rewrite Heqo. eauto.
+  SSSSSCase "regsat".
+  intros; destruct (peq res0 r); [subst | ].
+  SSSSSSCase "res = r".
+  unfold regsat, valsat. rewrite Regmap.gss.
+  destruct (zeq b b); [merge|congruence].
+  eapply RegMap.get_ge. eauto. apply RegMap.get_add_same. apply PTSet.In_singleton.
+  SSSSSSCase "res <> r".
+  unfold regsat, valsat. rewrite Regmap.gso; [|auto]. destruct (rs#r) as []_eqn; auto.
+  regsat_intro rs r. destruct (zeq b0 b).
+  SSSSSSSCase "b0 = b".
+  subst. eapply RegMap.get_ge. eauto. destruct (abs b) as []_eqn.
+  SSSSSSSSCase "abs b = Some".
+  exfalso. eapply Mem.fresh_block_alloc; eauto. apply MEM. congruence.
+  SSSSSSSSCase "abs b = None".
+  eapply RegMap.get_ge. apply RegMap.ge_add. apply IN. apply PTSet.In_top.
+  SSSSSSSCase "b0 <> b".
+  destruct (abs b0) as []_eqn.
+  SSSSSSSSCase "abs b0 = Some".
+  eapply RegMap.get_ge. eauto. eapply RegMap.get_ge. apply RegMap.ge_add. auto.
+  SSSSSSSSCase "abs b0 = None".
+  eapply PTSet.ge_trans. apply RegMap.get_ge. eauto.
+  eapply PTSet.ge_trans. apply RegMap.get_ge. apply RegMap.ge_add. auto.
+  SSSSSCase "memsat".
+  eapply memsat_ge; eauto.
+  unfold memsat, valsat in *. intros.
+  destruct (zeq b0 b).
+  SSSSSSCase "b0 = b".
+  subst. destruct v; auto. simpl in LOAD. pose proof LOAD as LOAD'.
+  eapply Mem.load_pointer_store in LOAD; eauto. intuition; try solve [congruence]; merge.
+  simpl in H0. pose proof (Int.unsigned_range o). omegaContradiction.
+  erewrite Mem.load_store_other in LOAD'; eauto.
+  eapply Mem.load_alloc_same in LOAD'; eauto. inv LOAD'.
+  SSSSSSCase "b0 <> b".
+  simpl in *.
+  erewrite Mem.load_store_other in LOAD; eauto.
+  erewrite Mem.load_alloc_unchanged in LOAD; eauto.
+  specialize (MSAT _ _ _ LOAD). destruct (abs b0) as []_eqn; auto.
+  destruct v; auto. destruct (zeq b1 b); auto.
+  subst. destruct (abs b) as []_eqn.
+  SSSSSSSSCase "abs b = Some".
+  exfalso. eapply Mem.fresh_block_alloc; eauto. apply MEM. congruence.
+  SSSSSSSSCase "abs b = None".
+  apply MSAT. apply PTSet.In_top.
+  SSSSSSCase "b0 <> b".
+  apply MEM. erewrite load_alloc_other' in LOAD; eauto.
+  specialize (MSAT _ _ _ LOAD). destruct (abs b0); auto; congruence.
+  SSSCase "EF_free".
+  exists abs. constructor; auto.
+  SSSSCase "ok_stack".
+  erewrite Mem.nextblock_free; eauto.
+  SSSSCase "ok_abs_mem".
+  eapply ok_abs_mem_free; eauto.
+  SSSSCase "ok_abs_result".
+  econstructor.
+  SSSSSCase "result".
+  unfold analysis. rewrite Heqo. eauto.
+  SSSSSCase "regsat".
+  intros; destruct (peq res0 r); [subst | eapply regsat_assign_other; eauto;
+    eapply regsat_ge; [eauto | eapply RegMap.ge_trans; eauto]].
+  unfold regsat, valsat. rewrite Regmap.gss. auto.
+  SSSSSCase "memsat".
+  eapply memsat_ge; eauto. eapply memsat_free; eauto.
+  SSSCase "EF_memcpy".
+  exists abs. constructor; auto.
+  SSSSCase "ok_stack".
+  erewrite Mem.nextblock_storebytes; eauto.
+  SSSSCase "ok_abs_mem".
+  eapply ok_abs_mem_storebytes; eauto.
+  SSSSCase "ok_abs_result".
+  econstructor.
+  SSSSSCase "result".
+  unfold analysis. rewrite Heqo. eauto.
+  SSSSSCase "regsat".
+  intros; destruct (peq res0 r); [subst | eapply regsat_assign_other; eauto;
+    eapply regsat_ge; [eauto | eapply RegMap.ge_trans; eauto]].
+  unfold regsat, valsat. rewrite Regmap.gss. auto.
+  SSSSSCase "memsat".
+  eapply memsat_ge; eauto.
+  unfold memsat, valsat in *. intros.
+  repeat (destruct args; try solve [inv H]). inv H. inv H0.
+  destruct (zeq b bdst).
+  SSSSSSCase "b = bdst".
+  subst. regsat_intro rs r. destruct (abs bdst) as []_eqn.
+  SSSSSSSCase "abs bdst = Some".
+  destruct v; auto. destruct (abs b) as []_eqn.
+  SSSSSSSSCase "abs b = Some".
+  apply In_add_ptset_to_image. apply PTSet.In_top. eapply In_unknown_offset; eauto.
+  SSSSSSSSCase "abs b = None".
+  eapply PTSet.ge_trans. repeat intro. apply In_add_ptset_to_image. apply H.
+  eapply In_unknown_offset; eauto. apply PTSet.ge_refl.
+  SSSSSSSCase "abs bdst = None".
+  eapply Mem.load_valid_access in LOAD. eapply Mem.valid_access_implies in LOAD.
+  eapply Mem.valid_access_valid_block in LOAD.
+  eapply Mem.storebytes_valid_block_2 in LOAD; eauto.
+  apply MEM in LOAD. congruence. constructor.
+  SSSSSSCase "b <> bdst".
+  specialize (MSAT b o v). feed MSAT. simpl. erewrite <- Mem.load_storebytes_other; eauto.
+  destruct (abs b); [|contradiction]. destruct v; auto. destruct (abs b0).
+  SSSSSSSCase "abs b0 = Some".
+  now apply MGE'.
+  SSSSSSSCase "abs b0 = None".
+  eapply PTSet.ge_trans. apply ge_add_ptset_to_image. auto.
+  SSSCase "EF_annot".
+  exists abs. constructor; auto.
+  SSSSCase "ok_abs_result".
+  econstructor.
+  SSSSSCase "result".
+  unfold analysis. rewrite Heqo. eauto.
+  SSSSSCase "regsat".
+  intros; destruct (peq res0 r); [subst | eapply regsat_assign_other; eauto;
+    eapply regsat_ge; [eauto | eapply RegMap.ge_trans; eauto]].
+  unfold regsat, valsat. rewrite Regmap.gss. auto.
+  SSSSSCase "memsat".
+  eapply memsat_ge; eauto.
+  SSSCase "EF_annot_val".
+  exists abs. constructor; auto.
+  SSSSCase "ok_abs_result".
+  econstructor.
+  SSSSSCase "result".
+  unfold analysis. rewrite Heqo. eauto.
+  SSSSSCase "regsat".
+  intros; destruct (peq res0 r); [subst | eapply regsat_assign_other; eauto;
+    eapply regsat_ge; [eauto | eapply RegMap.ge_trans; eauto]].
+  unfold regsat, valsat. rewrite Regmap.gss. destruct v; auto.
+  inv H1. specialize (GENV _ _ H5). rewrite GENV.
+  destruct args. inv H. destruct args; inv H. inv H0.
+  regsat_intro rs r0. rewrite GENV in IN.
+  eapply RegMap.get_ge. eauto. apply RegMap.get_add_same. auto.
+  SSSSSCase "memsat".
+  eapply memsat_ge; eauto. eapply MemMap.ge_trans; eauto.
+  SCase "Kildall failed".
+  rewrite PMap.gi in RPC. inv RPC.
+  inv STEP; try solve [
+    exists abs; constructor; auto; econstructor; eauto;
+      unfold analysis; rewrite Heqo; rewrite PMap.gi; reflexivity
+  ].
+  SSCase "Iop".
+  exists abs; constructor; auto.
+  SSSCase "ok_abs_result".
+  econstructor.
+  SSSSCase "result".
+  unfold analysis. rewrite Heqo. rewrite PMap.gi. reflexivity.
+  SSSSCase "regsat".
+  apply regsat_top.
+  SSSSCase "memsat".
+  apply memsat_top. auto.
+  SSCase "Iload".
+  exists abs; constructor; auto.
+  SSSCase "ok_abs_result".
+  econstructor.
+  SSSSCase "result".
+  unfold analysis. rewrite Heqo. rewrite PMap.gi. reflexivity.
+  SSSSCase "regsat".
+  apply regsat_top.
+  SSSSCase "memsat".
+  apply memsat_top. auto.
+  SSCase "Istore".
+  destruct a; try solve [inv H14].
+  exists abs; constructor; auto.
+  SSSCase "ok_stack".
+  erewrite Mem.nextblock_store; eauto.
+  SSSCase "ok_abs_mem".
+  eapply ok_abs_mem_store; eauto.
+  SSSCase "ok_abs_result".
+  econstructor.
+  SSSSCase "result".
+  unfold analysis. rewrite Heqo. rewrite PMap.gi. reflexivity.
+  SSSSCase "regsat".
+  apply regsat_top.
+  SSSSCase "memsat".
+  apply memsat_top. eapply ok_abs_mem_store; eauto.
+  SSCase "Ibuiltin".
+  destruct ef; inv H13; merge; try solve [
+    exists abs; constructor; auto; econstructor;
+    [ unfold analysis; rewrite Heqo; rewrite PMap.gi; reflexivity
+    | apply regsat_top
+    | apply memsat_top; auto
+    ]
+  ].
+  inv H0.
+  SSSCase "EF_vstore (volatile)".
+  exists abs. constructor; auto.
+  SSSSCase "ok_abs_result".
+  econstructor.
+  SSSSSCase "result".
+  unfold analysis. rewrite Heqo. rewrite Regmap.gi. reflexivity.
+  SSSSSCase "regsat".
+  apply regsat_top.
+  SSSSSCase "memsat".
+  apply memsat_top. auto.
+  SSSCase "EF_vstore (not volatile)".
+  exists abs. constructor; auto.
+  SSSSCase "ok_stack".
+  erewrite Mem.nextblock_store; eauto.
+  SSSSCase "ok_abs_mem".
+  eapply ok_abs_mem_store; eauto.
+  SSSSCase "ok_abs_result".
+  econstructor.
+  SSSSSCase "result".
+  unfold analysis. rewrite Heqo. rewrite Regmap.gi. reflexivity.
+  SSSSSCase "regsat".
+  apply regsat_top.
+  SSSSSCase "memsat".
+  apply memsat_top. eapply ok_abs_mem_store; eauto.
+  SSSCase "EF_vstore_global".
+  exists abs. inv H1; constructor; auto.
+  econstructor.
+  unfold analysis. rewrite Heqo. rewrite Regmap.gi. reflexivity.
+  apply regsat_top.
+  apply memsat_top. auto.
+  erewrite Mem.nextblock_store; eauto.
+  eapply ok_abs_mem_store; eauto.
+  econstructor.
+  unfold analysis. rewrite Heqo. rewrite Regmap.gi. reflexivity.
+  apply regsat_top.
+  apply memsat_top. eapply ok_abs_mem_store; eauto.
+  SSSCase "EF_malloc".
+  exists (fun x => if zeq x b then Some (Alloc pc) else abs x).
+  (* We will need this twice, so let's prove it upfront... *)
+  assert (OKAM:
+    ok_abs_mem
+    (fun x : Z => if zeq x b then Some (Alloc pc) else abs x)
+    m0).
+  unalias. split; intros.
+  destruct (zeq b0 b); [subst|].
+  eapply Mem.store_valid_block_1; eauto. eapply Mem.valid_new_block; eauto.
+  eapply Mem.store_valid_block_1; eauto. eapply Mem.valid_block_alloc; eauto.
+  apply MEM. auto.
+  destruct (zeq b0 b); [subst|].
+  congruence.
+  apply MEM.
+  eapply Mem.store_valid_block_2 in H2; [|eauto].
+  eapply Mem.valid_block_alloc_inv in H2; [|eauto].
+  inv H2. congruence. auto.
+  constructor; auto.
+  SSSSCase "ok_stack".
+  erewrite Mem.nextblock_store; [|eauto]. eapply ok_stack_alloc; eauto.
+  SSSSCase "ok_abs_genv".
+  unalias; intros. destruct (zeq b0 b); auto.
+  exfalso. subst. eapply Mem.fresh_block_alloc; eauto. apply MEM.
+  erewrite GENV; [congruence|eauto].
+  SSSSCase "sp".
+  destruct (zeq bsp b); auto.
+  subst. exfalso. eapply Mem.fresh_block_alloc; eauto. apply MEM. congruence.
+  SSSSCase "ok_abs_result".
+  econstructor.
+  SSSSSCase "result".
+  unfold analysis. rewrite Heqo. rewrite PMap.gi. reflexivity.
+  SSSSSCase "regsat".
+  apply regsat_top.
+  SSSSSCase "memsat".
+  apply memsat_top. auto.
+  SSSCase "EF_free".
+  exists abs. constructor; auto.
+  SSSSCase "ok_stack".
+  erewrite Mem.nextblock_free; eauto.
+  SSSSCase "ok_abs_mem".
+  eapply ok_abs_mem_free; eauto.
+  SSSSCase "ok_abs_result".
+  econstructor.
+  SSSSSCase "result".
+  unfold analysis. rewrite Heqo. rewrite PMap.gi. reflexivity.
+  SSSSSCase "regsat".
+  apply regsat_top.
+  SSSSSCase "memsat".
+  apply memsat_top. eapply ok_abs_mem_free; eauto.
+  SSSCase "EF_memcpy".
+  exists abs. constructor; auto.
+  SSSSCase "ok_stack".
+  erewrite Mem.nextblock_storebytes; eauto.
+  SSSSCase "ok_abs_mem".
+  eapply ok_abs_mem_storebytes; eauto.
+  SSSSCase "ok_abs_result".
+  econstructor.
+  SSSSSCase "result".
+  unfold analysis. rewrite Heqo. rewrite PMap.gi. reflexivity.
+  SSSSSCase "regsat".
+  apply regsat_top.
+  SSSSSCase "memsat".
+  apply memsat_top.
+  eapply ok_abs_mem_storebytes; eauto.
+
+  Case "state -> callstate".
+  exists abs. inv STEP.
+  SCase "Icall".
+  constructor; auto.
+  SSCase "ok_stack".
+  econstructor; eauto.
+  SSSCase "MEM".
+  apply MEM.
+  SSSCase "ok_abs_result_stack".
+  unfold analysis in RPC. destruct (failure_prone_analysis f) as []_eqn.
+  SSSSCase "Kildall terminated".
+  pose proof Heqo as FPS.
+  eapply Solver.fixpoint_solution with (n:=pc)(s:=pc') in FPS; [|
+    unfold successors; unfold successors_list; rewrite PTree.gmap1;
+      rewrite H6; simpl; auto; eapply list_nth_z_in; eauto].
+  unfold transf in FPS. rewrite H6 in FPS. unfold Solver.L.ge in FPS.
+  destruct (t#pc') as [rmap' mmap']_eqn. rewrite RPC in FPS. destruct FPS as [RGE MGE].
+  econstructor.
+  SSSSSCase "result".
+  unfold analysis. rewrite Heqo. eauto.
+  SSSSSCase "regsat".
+  eapply regsat_ge; eauto. eapply RegMap.ge_trans; eauto. apply RegMap.ge_add.
+  SSSSSCase "ret".
+  eapply PTSet.ge_trans. apply RegMap.get_ge; eauto.
+  eapply PTSet.ge_trans. apply RegMap.get_add_same. apply PTSet.ge_refl.
+  SSSSSCase "mem".
+  easy.
+  SSSSCase "Kildall failed".
+  econstructor.
+  SSSSSCase "result".
+  unfold analysis. rewrite Heqo. rewrite PMap.gi. eauto.
+  SSSSSCase "regsat".
+  eapply regsat_ge; eauto. apply RegMap.ge_top.
+  SSSSSCase "ret".
+  apply RegMap.get_top.
+  SSSSSCase "mem".
+  apply MemMap.ge_refl.
+  SCase "Itailcall".
+  constructor; auto.
+  SSCase "ok_abs_mem".
+  eapply ok_abs_mem_free; eauto.
+  SSCase "ok_stack".
+  erewrite Mem.nextblock_free; eauto.
+
+  Case "state -> returnstate".
+  exists abs. inv STEP.
+  constructor; auto.
+  SCase "ok_abs_mem".
+  eapply ok_abs_mem_free; eauto.
+  SCase "ok_stack".
+  erewrite Mem.nextblock_free; eauto.
+
+  Case "callstate -> state".
+  inv STEP.
+  exists (fun b =>
+    if zeq b stk then Some Stack else
+      match abs b with
+      | Some ab => Some (
+          match ab with
+          | Global i => Global i
+          | Globals  => Globals
+          | _        => Other
+          end
+        )
+      | None    => None
+      end
+  ).
+  constructor; auto.
+  SCase "ok_stack".
+  eapply ok_stack_alloc; eauto.
+  SCase "ok_abs_mem".
+  unalias; split; intros.
+  SSCase "->".
+  destruct (zeq b stk).
+  SSSCase "b = stk".
+  subst. eapply Mem.valid_new_block; eauto.
+  SSSCase "b <> stk".
+  destruct (abs b) as []_eqn; [|congruence].
+  eapply Mem.valid_block_alloc; eauto. apply MEM. congruence.
+  SSCase "<-".
+  destruct (zeq b stk).
+  SSSCase "b = stk".
+  congruence.
+  SSSCase "b <> stk".
+  destruct (abs b) as []_eqn. destruct a; congruence.
+  eapply Mem.valid_block_alloc_inv in H; eauto. intuition. apply MEM in H1; auto.
+  SCase "ok_abs_genv".
+  unalias; intros. specialize (GENV _ _ FIND). rewrite GENV.
+  destruct (zeq b stk); [|auto]. subst.
+  exfalso. eapply Mem.fresh_block_alloc; eauto. apply MEM. congruence.
+  SCase "sp".
+  destruct (zeq stk stk); [auto|congruence].
+  SCase "ok_abs_result".
+  destruct (failure_prone_analysis f0) as []_eqn.
+  SSCase "Kildall will terminate".
+  destruct t. destruct t. pose proof Heqo as FA.
+  eapply Solver.fixpoint_entry in Heqo; [|constructor; eauto].
+  destruct ((t, t1, t0) # (fn_entrypoint f0)) as [rmap mmap]_eqn.
+  setoid_rewrite Heqp in Heqo. unfold entry_result in Heqo.
+  destruct Heqo as [RGE MGE].
+  econstructor.
+  SSSCase "result".
+  unfold analysis. rewrite FA. eauto.
+  SSSCase "regsat".
+  eapply regsat_ge; eauto.
+  generalize (fn_params f0). intros. unalias.
+  destruct ((init_regs args l)#r) as []_eqn; auto.
+  assert (In r l).
+  SSSSCase "assert".
+  revert Heqv. revert args. induction l; intros.
+  simpl in Heqv. rewrite Regmap.gi in Heqv. congruence.
+  simpl in Heqv. destruct args.
+  rewrite Regmap.gi in Heqv. congruence.
+  destruct (peq r a).
+  subst. constructor. auto.
+  rewrite Regmap.gso in Heqv; [|auto]. right. eapply IHl; eauto.
+  SSSSCase "end of assert".
+  unfold entry_rmap. destruct (zeq b stk).
+  subst.
+  eapply fold_left_adds_prop; eauto; intros.
+  apply RegMap.get_add_same. apply PTSet.In_top.
+  now apply RegMap.ge_add.
+  destruct (abs b).
+  eapply fold_left_adds_prop; eauto; intros.
+  apply RegMap.get_add_same. apply PTSet.In_top.
+  now apply RegMap.ge_add.
+  eapply fold_left_adds_prop; eauto; intros.
+  apply RegMap.get_add_same.
+  eapply PTSet.ge_trans; eauto. now apply RegMap.ge_add.
+  SSSCase "memsat".
+  eapply memsat_ge; eauto. unalias. intros. destruct (zeq b stk).
+  SSSSCase "b = stk".
+  subst. simpl in LOAD. eapply Mem.load_alloc_same in LOAD; eauto. subst. auto.
+  SSSSCase "b <> stk".
+  destruct (abs b) as []_eqn.
+  SSSSSCase "abs b = Some".
+  destruct v; auto.
+  destruct (zeq b0 stk).
+  SSSSSSCase "b0 = stk".
+  subst. unfold entry_mmap.
+  apply MemMap.get_add_lt. destruct a; simpl; tauto. apply PTSet.In_top.
+
+  SSSSSSCase "b0 <> stk".
+  destruct (abs b0) as []_eqn.
+  SSSSSSSCase "abs b0 = Some".
+  unfold entry_mmap.
+  apply MemMap.get_add_lt. destruct a; simpl; tauto. apply PTSet.In_top.
+  SSSSSSSCase "abs b0 = None".
+  unfold entry_mmap. apply MemMap.get_add_lt. destruct a; simpl; tauto.
+  SSSSSCase "abs b = None".
+  eapply load_valid_block in LOAD. eapply Mem.valid_block_alloc_inv in LOAD; eauto.
+  intuition. apply MEM in H; auto.
+  SSCase "Kildall won't terminate".
+  econstructor; intros.
+  SSSCase "result".
+  unfold analysis. rewrite Heqo. rewrite PMap.gi. auto.
+  SSSCase "regsat".
+  unalias.
+  destruct ((init_regs args (fn_params f0))#r); auto.
+  destruct (zeq b stk).
+  subst. apply RegMap.get_top. apply PTSet.In_top.
+  destruct (abs b); apply RegMap.get_top; apply PTSet.In_top.
+  SSSCase "memsat".
+  unalias. intros. destruct (zeq b stk).
+  SSSSCase "b = stk".
+  subst. destruct v; auto. simpl in LOAD. eapply Mem.load_alloc_same in LOAD; eauto.
+  congruence.
+  SSSSCase "b <> stk".
+  destruct (abs b) as []_eqn.
+  SSSSSCase "abs b = Some".
+  destruct v; auto.
+  destruct (zeq b0 stk).
+  SSSSSSCase "b0 = stk".
+  subst. apply MemMap.get_top. apply PTSet.In_top.
+  SSSSSSCase "b0 <> stk".
+  destruct (abs b0) as []_eqn.
+  apply MemMap.get_top. apply PTSet.In_top.
+  apply MemMap.get_top.
+  SSSSSCase "abs b = None".
+  eapply load_valid_block in LOAD. eapply Mem.valid_block_alloc_inv in LOAD; eauto.
+  intuition. apply MEM in H; auto.
+
+  Case "callstate -> returnstate (un-inlined external calls)".
+  inv STEP. destruct ef; inv H4; try solve [exists abs; constructor; auto].
+  SCase "volatile store".
+  exists abs; constructor; auto.
+  inv H. auto. eapply ok_abs_mem_store; eauto.
+  inv H. auto. erewrite Mem.nextblock_store; eauto.
+  SCase "global volatile store".
+  exists abs; constructor; auto.
+  inv H0. auto. eapply ok_abs_mem_store; eauto.
+  inv H0. auto. erewrite Mem.nextblock_store; eauto.
+  SCase "malloc".
+  exists (fun x => if zeq x b then Some Other else abs x).
+  constructor; auto.
+  SSCase "ok_abs_mem".
+  constructor; intros.
+  destruct (zeq b0 b).
+  subst. eapply Mem.store_valid_block_1; eauto. eapply Mem.valid_new_block; eauto.
+  eapply Mem.store_valid_block_1; eauto. eapply Mem.valid_block_alloc; eauto. apply MEM.
+  auto.
+  destruct (zeq b0 b).
+  congruence.
+  apply MEM. eapply Mem.store_valid_block_2 in H1; [|eauto].
+  eapply Mem.valid_block_alloc_inv in H1; eauto.
+  intuition.
+  SSCase "ok_stack".
+  erewrite Mem.nextblock_store; [|eauto]. eapply ok_stack_alloc; eauto.
+  SSCase "ok_abs_genv".
+  unalias; intros. specialize (GENV _ _ FIND). destruct (zeq b0 b); [|auto].
+  subst. exfalso. eapply Mem.fresh_block_alloc; eauto. apply MEM. congruence.
+  SCase "free".
+  exists abs; constructor; auto.
+  SSCase "ok_abs_mem".
+  eapply ok_abs_mem_free; eauto.
+  SSCase "ok_stack".
+  erewrite Mem.nextblock_free; eauto.
+  SCase "memcpy".
+  exists abs; constructor; auto.
+  SSCase "ok_abs_mem".
+  constructor; intros.
+  eapply Mem.storebytes_valid_block_1; eauto. apply MEM. auto.
+  apply MEM. eapply Mem.storebytes_valid_block_2; eauto.
+  erewrite Mem.nextblock_storebytes; eauto.
+
+  Case "returnstate -> state".
+  inv STEP.
+  clear MEM GENV abs. (* don't even think about using this abs! *)
+  inv STK. (* use this good old abs instead! *)
+  exists (fun b =>
+    match abs b with
+    | Some _ => abs b
+    | None   => if (zlt b (Mem.nextblock m0)) then Some Other else None
+    end).
+  econstructor; eauto; intros.
+  SCase "ok_abs_mem".
+  constructor; intros.
+  specialize (MEM b). destruct (abs b). red. apply MEM. auto.
+  destruct (zlt b (Mem.nextblock m0)). auto. congruence.
+  destruct (abs b) as []_eqn. congruence.
+  destruct (zlt b (Mem.nextblock m0)); congruence.
+  SCase "ok_abs_genv".
+  unalias; intros. specialize (GENV _ _ FIND). rewrite GENV. auto.
+  SCase "sp".
+  rewrite SP. auto.
+  SCase "ok_abs_result".
+  inv RES.
+  econstructor; eauto; intros.
+  SSCase "regsat".
+  unalias. destruct (peq res r); [subst|].
+  SSSCase "res = r".
+  rewrite Regmap.gss. destruct v; auto.
+  destruct (abs b). apply RET. apply PTSet.In_top.
+  destruct (zlt b (Mem.nextblock m0)); [|auto].
+  apply RET. apply PTSet.In_top.
+  SSSCase "res <> r".
+  specialize (RSAT r). rewrite Regmap.gso; [|auto]. destruct (rs0#r); auto.
+  destruct (abs b). auto.
+  destruct (zlt b (Mem.nextblock m0)); [|auto].
+  apply RSAT. apply PTSet.In_top.
+  SSCase "memsat".
+  unalias. intros. destruct (abs b). destruct v0; auto.
+  destruct (abs b0); destruct (zlt b0 (Mem.nextblock m0));
+  repeat intro; apply MTOP; apply MemMap.get_top; apply PTSet.In_top.
+  destruct (zlt b (Mem.nextblock m0)). destruct v0; auto.
+  destruct (abs b0).
+  apply MTOP; apply MemMap.get_top; apply PTSet.In_top.
+  destruct (zlt b0 (Mem.nextblock m0));
+  repeat intro; apply MTOP; apply MemMap.get_top; apply PTSet.In_top.
+  apply load_valid_block in LOAD. congruence.
+Qed.
